start7

pset07_Subtyping/Pset7.v
@@ -44,6 +44,7 @@ Inductive value : exp -> Prop :=
 | VTupleNil : value TupleNil
 | VTupleCons : forall e1 e2, value e1 -> value e2 -> value (TupleCons e1 e2)
 .
+Local Hint Constructors value : core.
 
 (* The next few definitions are quite routine and should be safe to skim through
  * quickly; but start paying more attention when we get to defining the
@@ -91,6 +92,8 @@ Inductive plug : context -> exp -> exp -> Prop :=
     plug C e e'
     -> plug (Proj1 C n) e (Proj e' n)
 .
+Local Hint Constructors plug: core.
+
 
 (* Small-step, call-by-value evaluation *)
 Inductive step0 : exp -> exp -> Prop :=
@@ -110,6 +113,7 @@ Inductive step0 : exp -> exp -> Prop :=
     -> value v2
     -> step0 (Proj (TupleCons v1 v2) (1 + n)) (Proj v2 n)
 .
+Local Hint Constructors step0 : core.
 
 Inductive step : exp -> exp -> Prop :=
 | StepRule : forall C e1 e2 e1' e2',
@@ -117,6 +121,7 @@ Inductive step : exp -> exp -> Prop :=
     -> plug C e2 e2'
     -> step0 e1 e2
     -> step e1' e2'.
+Local Hint Constructors step : core.
 
 Definition trsys_of (e : exp) :=
   {| Initial := {e}; Step := step |}.
@@ -127,6 +132,7 @@ Inductive type :=
 | TupleTypeNil
 | TupleTypeCons (t1 t2 : type)
 .
+Local Hint Constructors type : core.
 
 Inductive subtype : type -> type -> Prop :=
 
@@ -170,6 +176,7 @@ Inductive proj_t : type -> nat -> type -> Prop :=
     proj_t t2 n t ->
     proj_t (TupleTypeCons t1 t2) (1 + n) t
 .
+Local Hint Constructors proj_t : core.
 
 (* Expression typing relation stating something _has_ a _ty_pe *)
 Inductive has_ty : fmap var type -> exp -> type -> Prop :=
@@ -201,6 +208,8 @@ Inductive has_ty : fmap var type -> exp -> type -> Prop :=
     t' $<: t ->
     has_ty G e t
 .
+Local Hint Constructors has_ty : core.
+
 
 (* Before we get started proving properties of our type system, please read
  * Pset7Sig.v and consider the questions below. This task is ungraded,
@@ -210,9 +219,15 @@ Inductive has_ty : fmap var type -> exp -> type -> Prop :=
  What does it mean for the subtyping order of the arguments in `StFun` to be 
  reversed?
 
+ Functions have contravariant subtyping. Intuitively, it makes sense that if the output of a function is t and t <: t', then the output can also be considered type t'.
+ But just because function's input can be type t and t <: t', that doesn't mean the
+ function is able to process values of type t', since there are things of type t'
+ but not of type t.
 
  If t1 $<: t2, what is known about some t3 that is a supertype of t2? And 
  likewise if it's a subtype of t1?
+
+ t1 <: t3. and t3 <: t2. In other words, transitivity
 
 
  How many goals do you get from calling `invert` on a hypothesis like
@@ -222,14 +237,24 @@ Inductive has_ty : fmap var type -> exp -> type -> Prop :=
  with the `LambdaCalculusAndTypeSoundness` definition of `has_ty`, and what 
  information do you have about `t`?
 
+  Only the HtAbs constructor can produce this, so invert produces a single goal. 
+ We get types t1 and t2 with t = Fun t1 t2, and the premise has_ty (G $+ (x, t1)) e1 t2
+ 
+ 
  To contrast, how many goals do you expect with the `has_ty` definition of
  this pset? Why is this the case? 
+
+ Here we have two goals. One is the same as the version from class, but the other one considers that the type of e1 is a subtype of the function's input type.
 
  Can you formulate a lemma that consolidates the information present in these 
  branches into one conclusion? (Imagine inverting now is equivalent to an
  "or" generating branches for each constructor; can you rephrase a lemma that
  leads to a conclusion with an "and" instead?)
 
+  forall G x e1 t,
+    has_ty G (Abs x e1) t ->
+    exists t1 t2,
+      has_ty (G $+ (x, t1)) e1 t2 /\ Fun t1 t2 $<: t.
 
  How many goals do you get from calling `invert` on a hypothesis like
  ```
@@ -238,11 +263,31 @@ Inductive has_ty : fmap var type -> exp -> type -> Prop :=
  with the `LambdaCalculusAndTypeSoundness` definition of `has_ty`, and what 
  information do you have about `e`? 
 
+3 goals. That's because there are three cases. We could've gotten a function because it was in the context as such. In that case, we know e is a variable. We could also have a function type since it's an abstraction. In that case, we know it's a lambda with type t1->t2. We could also get a function since e is some application App e1 e2, then we'd have that has_ty G e1 (Fun t_arg (Fun t1 t2)) and has_ty G e2 t_arg for some t_arg.
+
  To contrast, how many goals do you expect with the `has_ty` definition 
  of this pset? Why is this the case? 
 
- Can you formulate a lemma to recover information similar to what inverting
+ We also have all the same branches and two additional ones. First, we could've gotten the function from projecting out from a tuple. Second, we once again have the subtyping case.
+
+Can you formulate a lemma to recover information similar to what inverting
  gave you in FRAP's `has_ty` definition?
+
+  forall G e t1 t2,
+    has_ty G e (Fun t1 t2) ->
+    exists t1' t2',
+      has_ty G e (Fun t1' t2') /\
+      Fun t1' t2' $<: Fun t1 t2 /\
+      (forall x, e = Var x ->
+         G $? x = Some (Fun t1' t2')) /\
+      (forall x e1, e = Abs x e1 ->
+         has_ty (G $+ (x, t1')) e1 t2') /\
+      (forall e1 e2, e = App e1 e2 ->
+         exists t_arg,
+           has_ty G e1 (Fun t_arg (Fun t1' t2')) /\
+           has_ty G e2 t_arg) /\
+      (forall e' n, e = Proj e' n ->
+         exists t', has_ty G e' t' /\ proj_t t' n (Fun t1' t2')).
 
 *)
 
@@ -250,12 +295,12 @@ Inductive has_ty : fmap var type -> exp -> type -> Prop :=
 
 Lemma subtype_refl : forall t1, t1 $<: t1.
 Proof.
-Admitted.
+  induct t1; simplify.
+  - apply StFun; assumption.
+  - apply StTupleNilNil.
+  - apply StTupleCons; assumption.
+Qed.
 
-(* HINT 1 (see Pset7Sig.v) *) 
-Lemma subtype_trans : forall t1 t2 t3, t1 $<: t2 -> t2 $<: t3 -> t1 $<: t3.
-Proof.
-Admitted.
 
 (* BEGIN handy tactic that we suggest for these proofs *)
 Ltac tac0 :=
@@ -277,6 +322,44 @@ Ltac tac0 :=
 Ltac tac := simplify; subst; propositional; repeat (tac0; simplify); try equality.
 (* END handy tactic *)
 
+(* HINT 1 (see Pset7Sig.v) *) 
+
+Definition P (t1 t2 : type) : Prop :=
+  (forall t3, t2 $<: t3 -> t1 $<: t3)
+  /\ (forall t0, t0 $<: t1 -> t0 $<: t2).
+
+Lemma subtype_trans_aux : forall t1 t2, t1 $<: t2 -> P t1 t2.
+Proof.
+    simplify. 
+    induct H; 
+    unfold P; 
+    tac; eauto; 
+    unfold P in IHsubtype1, IHsubtype2; 
+    simplify; 
+    propositional; 
+    try (apply StFun; auto); 
+    try (apply StTupleCons; auto).
+    - invert H1; auto.
+Qed.
+
+Lemma subtype_trans : forall t1 t2 t3, t1 $<: t2 -> t2 $<: t3 -> t1 $<: t3.
+Proof.
+  simplify.
+  revert t3 H0.
+  induction H; intros t3 H23; invert H23; eauto.
+  rename t1' into a3.
+  rename t2' into b1.
+  rename t0 into a1.
+  rename t4 into b3.
+  rename t1 into a2.
+  rename t2 into b2.
+  pose proof (subtype_trans_aux).
+  pose proof (fun t1 t2 Hsub => proj1 (H1 t1 t2 Hsub)) as H_forward.
+  pose proof (fun t1 t2 Hsub => proj2 (H1 t1 t2 Hsub)) as H_backward.
+  apply StFun.
+  { apply H_forward with (t2 := a2); trivial. }
+  { auto. }
+Qed.
 
 (* The real prize: prove soundness of this type system.
  * We suggest starting from a copy of the type-safety proof from the book's
@@ -286,19 +369,263 @@ Ltac tac := simplify; subst; propositional; repeat (tac0; simplify); try equalit
  * task of this pset is to *extend* it to cover subtyping. This will involve
  * changing some proofs and making appropriate additional helper lemmas (there
  * are more hints in Pset7Sig.v).
- * Trying to write this proof from scratch is *not* recommended for this pset.
- * This is in contrast to the *previous* psets, which we tried to design so that
- * they could be solved from scratch with a good understanding of the lecture
- * material. *)
+*)
+
+Lemma canonical_fun :
+  forall G e t1 t2,
+    has_ty G e (Fun t1 t2) ->
+    value e ->
+    exists x e',
+      e = Abs x e'.
+Proof.
+    simplify. propositional. induct H.
+    - inversion H0.
+    - exists x, e1. propositional.
+    - inversion H1.
+    - inversion H1. 
+    - inversion H0.
+      apply IHhas_ty with (t1 := t1') (t2 := t2'); 
+      auto.
+Qed.
+
+Lemma canonical_tuple :
+  forall G e t1 t2,
+    has_ty G e (TupleTypeCons t1 t2) ->
+    value e ->
+    exists v1 v2,
+      e = TupleCons v1 v2 /\
+      value v1 /\ value v2.
+Proof.
+    simplify. propositional. induct H.
+    - inversion H0.
+    - inversion H1. 
+    - inversion H1. exists e1, e2. auto.
+    - inversion H1. 
+    - inversion H0. 
+      apply IHhas_ty with (t1 := t1') (t2 := t2'); auto.
+Qed.
+
+Lemma step_of_step0 :
+  forall e e', step0 e e' -> step e e'.
+Proof.
+  intros e e' Hstep0.
+  eapply StepRule with (C := Hole)
+                       (e1 := e) (e2 := e')
+                       (e1' := e) (e2' := e'); auto using PlugHole.
+Qed.
+Local Hint Resolve step_of_step0.
 
 (* HINT 2-3 (see Pset7Sig.v) *) 
-Theorem safety :
-  forall e t,
-    has_ty $0 e t -> invariantFor (trsys_of e)
-                                  (fun e' => value e'
-                                             \/ exists e'', step e' e'').
+Lemma progress : forall e t,
+    has_ty $0 e t
+    -> value e
+    \/ (exists e' : exp, step e e').
 Proof.
-Admitted.
+induct 1; eauto.
+- right. 
+  specialize (IHhas_ty1 eq_refl).
+  cases IHhas_ty1; cases IHhas_ty2. 
+  + pose proof (canonical_fun H IHhas_ty1). 
+    destruct H1 as [x [e' Heq]].
+    exists (subst e2 x e').
+    apply step_of_step0.
+    rewrite Heq. 
+    eauto. 
+  + destruct IHhas_ty2.
+    exists (App e1 x).
+    inversion H1. 
+    apply StepRule with (C :=  App2 e1 C) (e1 := e0) (e2 := e3);
+    auto. 
+  + destruct IHhas_ty1.
+    inversion H1.
+    exists (App x e2).
+    apply StepRule with (C := App1 C e2) (e1 := e0) (e2 := e3);
+    auto.
+  + destruct IHhas_ty1.
+    inversion H1.
+    exists (App x e2).
+    apply StepRule with (C := App1 C e2) (e1 := e0) (e2 := e3);
+    auto.
+- specialize (IHhas_ty1 eq_refl).
+  cases IHhas_ty1; cases IHhas_ty2.
+  + left; auto.
+  + right. 
+    destruct IHhas_ty2.
+    inversion H1. 
+    exists (TupleCons e1 x).
+    apply StepRule with (C := TupleCons2 e1 C) (e1 := e0) (e2 := e3); auto.
+  + right.
+    destruct IHhas_ty1.
+    inversion H1. 
+    exists (TupleCons x e2).
+    apply StepRule with (C := TupleCons1 C e2) (e1 := e0) (e2 := e3); auto.
+  + right.
+    destruct IHhas_ty1.
+    inversion H1. 
+    exists (TupleCons x e2).
+    apply StepRule with (C := TupleCons1 C e2) (e1 := e0) (e2 := e3); auto.
+- right.
+  invert H0;
+  cases IHhas_ty.
+  + pose proof (canonical_tuple) H IHhas_ty; 
+    destruct H0 as [v1 [v2 [Heq [val1 val2]]]].
+    exists v1. 
+    apply step_of_step0.
+    rewrite Heq.
+    auto.
+  + destruct IHhas_ty.
+    exists (Proj x 0).
+    inversion H0.
+    apply StepRule with (C := Proj1 C 0) (e1 := e1) (e2 := e2); 
+    auto. 
+  + pose proof (canonical_tuple) H IHhas_ty; 
+    destruct H0 as [v1 [v2 [Heq [val1 val2]]]].
+    exists (Proj v2 n0).
+    apply step_of_step0.
+    rewrite Heq.
+    auto.
+  + destruct IHhas_ty.
+    exists (Proj x (1 + n0)).
+    inversion H0.
+    apply StepRule with (C := Proj1 C (1 + n0)) (e1 := e1) (e2 := e2); 
+    auto. 
+Qed. 
+
+Lemma weakening_override : forall (G G' : fmap var type) x t,
+(forall x' t', G $? x' = Some t' -> G' $? x' = Some t')
+-> (forall x' t', G $+ (x, t) $? x' = Some t'
+                    -> G' $+ (x, t) $? x' = Some t').
+Proof.
+simplify.
+cases (x ==v x'); simplify; eauto.
+Qed.
+
+Local Hint Resolve weakening_override : core.
+
+Lemma weakening : forall G e t,
+has_ty G e t
+-> forall G', (forall x t, G $? x = Some t -> G' $? x = Some t)
+    -> has_ty G' e t.
+Proof.
+induct 1; simplify; tac; eauto 6.
+Qed.
+
+Local Hint Resolve weakening : core.
+
+(* Replacing a typing context with an equal one has no effect (useful to guide
+* proof search as a hint). *)
+Lemma has_ty_change : forall G e t,
+has_ty G e t
+-> forall G', G' = G
+    -> has_ty G' e t.
+Proof. tac. Qed.
+
+Local Hint Resolve has_ty_change : core.
+
+Lemma substitution : forall G x t' e t e',
+has_ty (G $+ (x, t')) e t
+-> has_ty $0 e' t'
+-> has_ty G (subst e' x e) t.
+Proof. induct 1; tac; eauto. Qed.
+Local Hint Resolve substitution : core.
+
+
+Lemma has_ty_TupleCons G e e' t:
+   has_ty G (TupleCons e e') t ->
+   exists t1 t2, has_ty G e t1 /\ has_ty G e' t2 /\ TupleTypeCons t1 t2 $<: t.
+Proof. Admitted.
+
+Lemma preservation0 : forall e1 e2,
+step0 e1 e2
+-> forall t, has_ty $0 e1 t
+    -> has_ty $0 e2 t.
+Proof.
+invert 1; tac.
+(* - eapply substitution.
+    + invert H.
+        * invert H4. {eapply H2. } *)
+(*
+Preservation proof runs by inversion on the primitive step and relies on the inversion lemmas for typing plus substitution and subtyping facts.
+
+Beta: From has_ty $0 (App (Abs x e) v) t, use the App inversion lemma (parallel to has_ty_TupleCons in Pset7.v:...) to get t1, t2, typings of the operands, and Fun t1 t2 $<: t. The Abs inversion lemma yields has_ty ($0 $+ (x, t1)) e t2; substitution gives has_ty $0 (subst v x e) t2, and the saved subtyping derivation lifts the result to t.
+
+Proj0: Projection inversion on has_ty $0 (Proj (TupleCons v1 v2) 0) t produces a witness TupleTypeCons t1 t2 $<: t; the tuple inversion lemma recovers typings for v1 and v2, and reflexivity of subtyping delivers has_ty $0 v1 t.
+
+ProjS: Projection inversion plus has_ty_TupleCons again expose types for the tuple components and the residual projection. Reassemble the typing derivation for Proj v2 n, then apply the collected subtyping proof to reach t.
+
+Each branch therefore constructs has_ty $0 e2 t, completing preservation for step0.
+*)
+invert H.
+    + invert H4; apply substitution with (t' := t1); auto.
+    
+        * apply substitution .
+ (* apply substitution with (t' := t1). *)
+    + invert H. 
+        * invert H4. { eapply H2. }
+info_eauto 6.
+Qed.
+(* 
+
+Local Hint Resolve preservation0 : core.
+
+Lemma preservation' : forall C e1 e1',
+    plug C e1 e1'
+    -> forall e2 e2' t, plug C e2 e2'
+    -> step0 e1 e2
+    -> has_ty $0 e1' t
+    -> has_ty $0 e2' t.
+Proof.
+induct 1; t.
+Qed.
+Local Hint Resolve preservation' : core.
+
+
+    HINT 3: Helper lemmas for preservation: Typing inversion
+In the proof of preservation for `step0`, you will have `has_ty` hypotheses for for expressions with known constructors, e.g. for an `(Abs x e)` or for a `(TupleCons e1 e2)` etc.
+Without subtyping, inverting such a `has_ty` would give you just one subgoal, where the `has_ty` is replaced by the preconditions that were used to construct it.
+Now, with subtyping, you get one additional subgoal for the `HtSub` case, where the original `has_ty` is replaced by a similar looking `has_ty` and a subtyping derivation. You could invert that new `has_ty` again, and again and again, and your proving endeavor would never end.
+This hint shows how to solve this problem for `TupleCons`, but you will have to apply this trick for all constructors of `exp`.
+Without subtyping, we would know that if `TupleCons e1 e2` has a type t, then there are some types t1 and t2 such that e1 has type t1, e2 has type t2, and `t = TupleTypeCons t1 t2`. This fact would follow directly from the fact that there is only a single rule for typing a TupleCons expression.
+However, once we add subtyping, the HtSub rule allows us to type an expression of any form, and so the above property doesn't hold. A typing derivation for the fact that `TupleCons e1 e2` has type t can be arbitrarily long even when e1 and e2 are small, but we still know that it must start from an application of the HtTupleCons rule, followed by potentially many applications of the HtSub rule. Since we have proven that the subtype relation is reflexive and transitive, we know the many applications of the HtSub rule can be replaced with exactly one, meaning we know that there is a derivation for TupleCons e1 e2 that is an HtSub rule applied to the HtTupleCons rule. This tells us the following fact:
+Lemma has_ty_TupleCons G e e' t:
+   has_ty G (TupleCons e e') t ->
+   exists t1 t2, has_ty G e t1 /\ has_ty G e' t2 /\ TupleTypeCons t1 t2 $<: t.
+Knowing this fact is useful for the type-safety proof, because now whenever we know that `TupleCons e e'` has some type, we can directly get information about the types of its subexpressions. If we only tried to invert the original typing derivation, the last rule in the derivation may have been HtSub, in which case we would make no "progress" down towards finding the application of the rule HtTupleCons.
+You should be able to formulate and prove similar lemmas for Abs, App, and Proj.
+
+
+   *)
+  Lemma preservation : forall e1 e2,
+    step e1 e2
+    -> forall t, has_ty $0 e1 t
+      -> has_ty $0 e2 t.
+  Proof.
+    admit.
+    (* invert 1; t. *)
+  Admitted.
+
+  Local Hint Resolve progress preservation : core.
+
+(* Theorem safety : forall e t, has_ty $0 e t
+    -> invariantFor (trsys_of e)
+                    (fun e' => value e'
+                               \/ exists e'', step e' e'').
+  Proof.
+    simplify.
+    apply invariant_weaken with (invariant1 := fun e' => has_ty $0 e' t); eauto.
+    apply invariant_induction; simplify; eauto; equality.
+  Qed. *)
+
+Theorem safety : forall e t, has_ty $0 e t
+  -> invariantFor (trsys_of e)
+                  (fun e' => value e'
+                            \/ exists e'', step e' e'').
+Proof.
+   simplify.
+    apply invariant_weaken with (invariant1 := fun e' => has_ty $0 e' t); eauto.
+    - apply invariant_induction; simplify; eauto.
+        + destruct H0; subst; auto. exfalso; auto.
+Qed.
 
 End Impl.
 
